Memory.thy
@@ -18,15 +18,15 @@ named_theorems single_memory_simps
 named_theorems single_memory_intro
 
 lemma single_memory_\<alpha>_set[single_memory_simps]:
-  assumes "single_memory_\<alpha> s a \<noteq> None"
-  shows "single_memory_\<alpha> (s[a := mem_val v]) = (single_memory_\<alpha> s)(a := Some (Some v))"
+  assumes "single_memory_\<alpha> s a \<noteq> None \<and> single_memory_\<alpha> s a \<noteq> Some mem_freed"
+  shows "single_memory_\<alpha> (s[a := mem_val v]) = (single_memory_\<alpha> s)(a := Some (mem_val v))"
   using assms
-  unfolding single_memory_\<alpha>_def valid_single_memory_address_def
+  unfolding single_memory_\<alpha>_def allocated_single_memory_address_def
   by (auto split: if_splits)
 
 lemma memory_\<alpha>_set_heap[simp]:
-  assumes "memory_\<alpha> (l,g,s,h) (haddr a) \<noteq> None"
-  shows "memory_\<alpha> (l,g,s,h[a := mem_val v]) = ((memory_\<alpha> (l,g,s,h))((haddr a) := Some (Some v)))"
+  assumes "memory_\<alpha> (l,g,s,h) (haddr a) \<noteq> None \<and> memory_\<alpha> (l,g,s,h) (haddr a) \<noteq> Some mem_freed"
+  shows "memory_\<alpha> (l,g,s,h[a := mem_val v]) = ((memory_\<alpha> (l,g,s,h))((haddr a) := Some (mem_val v)))"
   apply (rule ext)
   subgoal for a'
   using assms single_memory_simps
@@ -34,8 +34,8 @@ lemma memory_\<alpha>_set_heap[simp]:
   done
 
 lemma memory_\<alpha>_set_stack[simp]:
-  assumes "memory_\<alpha> (l,g,s,h) (saddr a) \<noteq> None"
-  shows "memory_\<alpha> (l,g,s[a := mem_val v],h) = ((memory_\<alpha> (l,g,s,h))((saddr a) := Some (Some v)))"
+  assumes "memory_\<alpha> (l,g,s,h) (saddr a) \<noteq> None \<and> memory_\<alpha> (l,g,s,h) (saddr a) \<noteq> Some mem_freed"
+  shows "memory_\<alpha> (l,g,s[a := mem_val v],h) = ((memory_\<alpha> (l,g,s,h))((saddr a) := Some (mem_val v)))"
   apply (rule ext)
   subgoal for a'
   using assms single_memory_simps
@@ -45,13 +45,13 @@ lemma memory_\<alpha>_set_stack[simp]:
 lemma single_memory_\<alpha>_allocate[single_memory_simps]:
   assumes "a \<noteq> length m"
   shows "single_memory_\<alpha> (m@[mem_unset]) a = (single_memory_\<alpha> m) a"
-  unfolding single_memory_\<alpha>_def valid_single_memory_address_def
+  unfolding single_memory_\<alpha>_def allocated_single_memory_address_def
   using assms
   by (auto simp: nth_append)
 
 lemma single_memory_\<alpha>_allocated[single_memory_simps]:
-  "single_memory_\<alpha> (m@[mem_unset]) (length m) = Some None"
-  unfolding single_memory_\<alpha>_def valid_single_memory_address_def
+  "single_memory_\<alpha> (m@[mem_unset]) (length m) = Some mem_unset"
+  unfolding single_memory_\<alpha>_def allocated_single_memory_address_def
   by simp
 
 lemma memory_\<alpha>_allocate_heap_eq:
@@ -67,62 +67,100 @@ lemma memory_\<alpha>_allocate_stack_eq:
   by (cases a; simp add: single_memory_simps)
 
 lemma memory_\<alpha>_allocate_heap[simp]:
-  "memory_\<alpha> (l, g, s, h @ [mem_unset]) = (memory_\<alpha> (l, g, s, h))(haddr (length h) := Some None)"
+  "memory_\<alpha> (l, g, s, h @ [mem_unset]) = (memory_\<alpha> (l, g, s, h))(haddr (length h) := Some mem_unset)"
   by (auto simp: memory_\<alpha>_allocate_heap_eq single_memory_simps)
 
 lemma memory_\<alpha>_allocate_stack[simp]:
-  "memory_\<alpha> (l, g, s @ [mem_unset], h) = (memory_\<alpha> (l, g, s, h))(saddr (length s) := Some None)"
+  "memory_\<alpha> (l, g, s @ [mem_unset], h) = (memory_\<alpha> (l, g, s, h))(saddr (length s) := Some mem_unset)"
   by (auto simp: memory_\<alpha>_allocate_stack_eq single_memory_simps)
 
 
 lemma single_memory_\<alpha>_free[single_memory_simps]:
-  "single_memory_\<alpha> (s[a := mem_freed]) = (single_memory_\<alpha> s)(a := None)"
-  unfolding single_memory_\<alpha>_def valid_single_memory_address_def
+  assumes "allocated_single_memory_address s a"
+  shows "single_memory_\<alpha> (s[a := mem_freed]) = (single_memory_\<alpha> s)(a := Some mem_freed)"
+  using assms
+  unfolding single_memory_\<alpha>_def allocated_single_memory_address_def
   by (auto split: if_splits)
 
 lemma memory_\<alpha>_free_heap[simp]:
-  "memory_\<alpha> (l,g,s,h[a := mem_freed]) = (memory_\<alpha> (l,g,s,h))(haddr a := None)"
+  assumes "allocated_memory_address (l,g,s,h) (haddr a)"
+  shows "memory_\<alpha> (l,g,s,h[a := mem_freed]) = (memory_\<alpha> (l,g,s,h))(haddr a := Some mem_freed)"
   apply (rule ext)
   subgoal for a'
+    using assms
     by (cases a'; simp add: single_memory_simps)
   done
 
 lemma memory_\<alpha>_free_stack[simp]:
-  "memory_\<alpha> (l,g,s[a := mem_freed],h) = (memory_\<alpha> (l,g,s,h))(saddr a := None)"
+  assumes "allocated_memory_address (l,g,s,h) (saddr a)"
+  shows "memory_\<alpha> (l,g,s[a := mem_freed],h) = (memory_\<alpha> (l,g,s,h))(saddr a := Some mem_freed)"
   apply (rule ext)
   subgoal for a'
+    using assms
     by (cases a'; simp add: single_memory_simps)
   done
 
 lemma single_memory_\<alpha>_not_none_iff[single_memory_simps]:
-  "valid_single_memory_address s a \<longleftrightarrow> single_memory_\<alpha> s a \<noteq> None"
+  "allocated_single_memory_address s a \<longleftrightarrow> single_memory_\<alpha> s a \<noteq> None"
   unfolding single_memory_\<alpha>_def valid_single_memory_address_def
   by (cases "s!a"; simp)
 
-lemma memory_\<alpha>_not_none_iff[simp]:
-  "valid_memory_address s a \<longleftrightarrow> memory_\<alpha> s a \<noteq> None"
+lemma allocated_address_iff[simp]:
+  "allocated_memory_address s a \<longleftrightarrow> memory_\<alpha> s a \<noteq> None"
   by (cases s; cases a; simp add: single_memory_simps)
 
-lemma memory_\<alpha>_allocate_validity[simp]:
-  assumes "memory_\<alpha> m' = (memory_\<alpha> m)(a := Some None)"
-  assumes "a \<noteq> a'"
-  shows "valid_memory_address m a' = valid_memory_address m' a' \<and> valid_memory_address m' a"
-  using assms
-  by simp
+lemma valid_address_iff[simp]:
+  "valid_memory_address s a \<longleftrightarrow> (memory_\<alpha> s a \<noteq> None \<and> memory_\<alpha> s a \<noteq> Some mem_freed)"
+  by (cases s; cases a; auto simp: single_memory_\<alpha>_def valid_single_memory_address_def)
 
-lemma memory_\<alpha>_set_validity[simp]:
-  assumes "memory_\<alpha> m' = (memory_\<alpha> m)(a := Some (Some v))"
-  assumes "memory_\<alpha> m a \<noteq> None"
-  shows "valid_memory_address m = valid_memory_address m'"
-  using assms
-  by (simp add: fun_eq_iff)
 
-lemma memory_\<alpha>_free_validity[simp]:
-  assumes "memory_\<alpha> m' = (memory_\<alpha> m)(a := None)"
-  assumes "a \<noteq> a'"
-  shows "valid_memory_address m a' = valid_memory_address m' a' \<and> \<not>valid_memory_address m' a"
+lemma memory_\<alpha>_allocate_validity:
+  assumes "memory_\<alpha> m' = (memory_\<alpha> m)(a := Some mem_unset)"
+  shows "allocated_memory_address m' = (allocated_memory_address m)(a := True)"
   using assms
-  by simp
+  by (auto simp: fun_eq_iff)
+
+
+lemma memory_\<alpha>_set_validity:
+  assumes "valid_memory_address s a"
+  assumes "memory_\<alpha> s' = (memory_\<alpha> s)(a := Some (mem_val v))"
+  shows "allocated_memory_address s' = allocated_memory_address s" "valid_memory_address s' = valid_memory_address s"
+  subgoal
+    apply (rule ext)
+    subgoal for addr
+      using assms
+      apply (cases s; cases s'; cases addr; cases "a = addr")
+      by (auto simp add: single_memory_\<alpha>_def valid_single_memory_address_def)
+  done
+  subgoal
+    apply (rule ext)
+    subgoal for addr
+      using assms
+      apply (cases s; cases s'; cases addr; cases "a = addr")
+      by (auto simp add: single_memory_\<alpha>_def fun_upd_def valid_single_memory_address_def fun_eq_iff allocated_single_memory_address_def split: if_splits)
+  done
+  done
+
+lemma memory_\<alpha>_free_validity:
+  assumes "valid_memory_address s a"
+  assumes "memory_\<alpha> s' = (memory_\<alpha> s)(a := Some mem_freed)"
+  shows "allocated_memory_address s' = allocated_memory_address s" "valid_memory_address s' = (valid_memory_address s)(a := False)"
+  subgoal
+    apply (rule ext)
+    subgoal for addr
+      using assms
+      apply (cases s; cases s'; cases addr)
+      by (auto simp: single_memory_\<alpha>_def valid_single_memory_address_def split: if_splits)
+    done
+  subgoal
+    apply (rule ext)
+    subgoal for addr
+      using assms
+      apply (cases s; cases s'; cases addr; cases "a = addr")
+      by (auto simp: single_memory_\<alpha>_def valid_single_memory_address_def allocated_single_memory_address_def fun_upd_def fun_eq_iff split: if_splits)
+    done
+  done
+
 
 lemma memory_\<alpha>_distinct_addresses[simp]:
   "memory_\<alpha> s a1 = Some v \<Longrightarrow> memory_\<alpha> s a2 = None \<Longrightarrow> a1 \<noteq> a2"
@@ -134,28 +172,28 @@ lemma memory_\<alpha>_distinct_addresses[simp]:
 section "memory_\<alpha> operations"
 
 lemma set_memory_\<alpha>:
-  assumes "memory_\<alpha> s a \<noteq> None"
-  shows "\<exists>s'. set_memory a v s = ok s' \<and> memory_\<alpha> s' = (memory_\<alpha> s)(a := Some (Some v))"
+  assumes "valid_memory_address s a"
+  shows "\<exists>s'. set_memory a v s = ok s' \<and> memory_\<alpha> s' = (memory_\<alpha> s)(a := Some (mem_val v))"
   using assms
-  by (cases s; cases a; auto simp: single_memory_\<alpha>_def set_single_memory_def split: if_splits)
+  by (cases s; cases a; auto simp: single_memory_\<alpha>_def set_single_memory_def valid_single_memory_address_def split: if_splits)
 
 lemma allocate_stack_\<alpha>:
   assumes "allocate_stack s = (s', a)"
-  shows "memory_\<alpha> s' = (memory_\<alpha> s)(a := Some None)"
+  shows "memory_\<alpha> s' = (memory_\<alpha> s)(a := Some mem_unset)"
   using assms
   by (cases s; cases s'; cases a; auto simp: allocate_stack_def allocate_single_memory_def)
 
 lemma allocate_heap_\<alpha>:
   assumes "allocate_heap s = (s', a)"
-  shows "memory_\<alpha> s' = (memory_\<alpha> s)(a := Some None)"
+  shows "memory_\<alpha> s' = (memory_\<alpha> s)(a := Some mem_unset)"
   using assms
   by (cases s; cases s'; cases a; auto simp: allocate_heap_def allocate_single_memory_def)
 
 lemma free_memory_\<alpha>:
-  assumes "memory_\<alpha> s a \<noteq> None"
-  shows "\<exists>s'. free_memory a s = ok s' \<and> memory_\<alpha> s' = (memory_\<alpha> s)(a := None)"
+  assumes "valid_memory_address s a"
+  shows "\<exists>s'. free_memory a s = ok s' \<and> memory_\<alpha> s' = (memory_\<alpha> s)(a := Some mem_freed)"
   using assms
-  by (cases s; cases a; auto simp: free_single_memory_def single_memory_\<alpha>_def split: if_splits)
+  by (cases s; cases a; auto simp: single_memory_\<alpha>_def free_single_memory_def valid_single_memory_address_def split: if_splits)
 
 
 
@@ -171,60 +209,60 @@ lemma wp_case_memory_value_intro[wp_intro]:
 
 
 lemma wp_get_single_memory_intro[THEN consequence, single_memory_intro]:
-  assumes "single_memory_\<alpha> s a \<noteq> None"
-  assumes "single_memory_\<alpha> s a \<noteq> Some None"
-  shows "wp (get_single_memory s a) (\<lambda>x. single_memory_\<alpha> s a = Some (Some x))"
+  assumes "valid_single_memory_address s a" "single_memory_\<alpha> s a \<noteq> Some mem_unset"
+  shows "wp (get_single_memory s a) (\<lambda>x. single_memory_\<alpha> s a = Some (mem_val x))"
   using assms
   unfolding get_single_memory_def valid_single_memory_address_def single_memory_\<alpha>_def
   by (intro wp_intro; simp)
 
 lemma wp_get_memory_intro[THEN consequence, wp_intro]:
-  assumes "memory_\<alpha> s a \<noteq> None"
-  assumes "memory_\<alpha> s a \<noteq> Some None"
-  shows "wp (get_memory s a) (\<lambda>x. memory_\<alpha> s a = Some (Some x))"
+  assumes "valid_memory_address s a" "memory_\<alpha> s a \<noteq> Some mem_unset"
+  shows "wp (get_memory s a) (\<lambda>x. memory_\<alpha> s a = Some (mem_val x))"
   using assms
-  by (cases a; cases s; simp; intro single_memory_intro; simp)
+  by (cases a; cases s; simp; intro single_memory_intro; simp add: single_memory_\<alpha>_def valid_single_memory_address_def split: if_splits)
 
 
 lemma wp_set_single_memory_intro[THEN consequence, single_memory_intro]:
-  assumes "single_memory_\<alpha> m a \<noteq> None"
-  shows "wp (set_single_memory a v m) (\<lambda>m'. single_memory_\<alpha> m' = (single_memory_\<alpha> m)(a := Some (Some v)))"
+  assumes "valid_single_memory_address s a"
+  shows "wp (set_single_memory a v s) (\<lambda>s'. single_memory_\<alpha> s' = (single_memory_\<alpha> s)(a := Some (mem_val v)))"
   using assms
   unfolding set_single_memory_def
-  by (intro wp_intro wp_return_intro; simp add: single_memory_simps)
-                                                                               
+  by (intro wp_intro wp_return_intro; simp add: single_memory_\<alpha>_def valid_single_memory_address_def allocated_single_memory_address_def fun_eq_iff split: if_splits)
+
+
 lemma wp_set_memory_intro[THEN consequence, wp_intro]:
-  assumes "memory_\<alpha> s a \<noteq> None"
-  shows "wp (set_memory a v s) (\<lambda>s'. memory_\<alpha> s' = (memory_\<alpha> s)(a := Some (Some v)) \<and> register_\<alpha> s = register_\<alpha> s')"
+  assumes "valid_memory_address s a"
+  shows "wp (set_memory a v s) (\<lambda>s'. memory_\<alpha> s' = (memory_\<alpha> s)(a := Some (mem_val v)) \<and> register_\<alpha> s = register_\<alpha> s')"
   using assms 
-  apply (cases a; cases s; simp)
-  unfolding set_single_memory_def
-  by (intro wp_intro wp_return_intro; simp add: single_memory_simps; rule ext; simp)+
+  by (cases a; cases s; simp add: set_single_memory_def; intro wp_intro wp_return_intro; simp add: single_memory_\<alpha>_def valid_single_memory_address_def allocated_single_memory_address_def fun_eq_iff split: if_splits; metis register_\<alpha>_eq)
 
 
 lemma wp_free_single_memory_intro[THEN consequence, single_memory_intro]:
-  assumes "single_memory_\<alpha> s a \<noteq> None"
-  shows "wp (free_single_memory a s) (\<lambda>s'. (single_memory_\<alpha> s') = (single_memory_\<alpha> s)(a := None))"
+  assumes "valid_single_memory_address s a"
+  shows "wp (free_single_memory a s) (\<lambda>s'. (single_memory_\<alpha> s') = (single_memory_\<alpha> s)(a := Some mem_freed))"
   using assms
   unfolding free_single_memory_def
   apply (intro wp_intro wp_return_intro)
-  apply (simp add: single_memory_simps)
-  by (simp add: single_memory_simps)
+  by (auto simp: single_memory_\<alpha>_free valid_single_memory_address_def)
 
 lemma wp_free_memory_intro[THEN consequence, wp_intro]:
-  assumes "memory_\<alpha> s a \<noteq> None"
-  shows "wp (free_memory a s) (\<lambda>s'. memory_\<alpha> s' = (memory_\<alpha> s)(a := None) \<and> register_\<alpha> s = register_\<alpha> s')"
-  using assms
+  assumes "valid_memory_address s a"
+  shows "wp (free_memory a s) (\<lambda>s'. memory_\<alpha> s' = (memory_\<alpha> s)(a := Some mem_freed) \<and> register_\<alpha> s = register_\<alpha> s')"
   apply (cases a; cases s; simp)
-  apply (intro wp_intro single_memory_intro wp_return_intro; simp; rule ext)
-  subgoal for _ _ _ _ _ _ a' by (cases a'; simp)
-  apply (intro wp_intro single_memory_intro wp_return_intro; simp; rule ext)
-  subgoal for _ _ _ _ _ _ a' by (cases a'; simp)
+  using assms
+  apply (intro wp_intro single_memory_intro wp_return_intro, auto) using assms 
+  using assms valid_memory_address.simps(2) apply blast
+   apply (rule ext)
+  subgoal for _ _ _ _ _ _ _ a' by (cases a'; simp)
+  apply (intro wp_intro single_memory_intro wp_return_intro, auto) using assms 
+  using assms valid_memory_address.simps apply blast
+   apply (rule ext)
+  subgoal for _ _ _ _ _ _ _ a' by (cases a'; simp)
   done
 
 
 lemma wp_allocate_single_memory[THEN consequence, single_memory_intro]:
-  "wp (return (allocate_single_memory s)) (\<lambda>(s', a). (single_memory_\<alpha> s') = (single_memory_\<alpha> s)(a := Some None) \<and> single_memory_\<alpha> s a = None)"
+  "wp (return (allocate_single_memory s)) (\<lambda>(s', a). (single_memory_\<alpha> s') = (single_memory_\<alpha> s)(a := Some mem_unset) \<and> single_memory_\<alpha> s a = None)"
   unfolding allocate_single_memory_def
   apply (intro wp_intro wp_return_intro; auto simp: single_memory_simps)
   by (simp add: single_memory_\<alpha>_def valid_single_memory_address_def)
@@ -240,5 +278,23 @@ lemma wp_allocate_stack_intro[THEN consequence, wp_intro]:
   unfolding allocate_stack_def allocate_single_memory_def
   apply (cases s; intro wp_intro wp_return_intro; auto)
   by (simp add: single_memory_\<alpha>_def valid_single_memory_address_def)
+
+
+
+section "Stack Frames"
+
+definition "mem_op_well_behaved f \<equiv> \<forall>s a. ((memory_\<alpha> s a \<noteq> None \<longrightarrow> memory_\<alpha> (f s) a \<noteq> None) \<and> (memory_\<alpha> s a = Some mem_freed \<longrightarrow> memory_\<alpha> (f s) a = Some mem_freed))"
+
+
+
+lemma "s' = push_frame s \<Longrightarrow> s'' = f s' \<Longrightarrow> mem_op_well_behaved f \<Longrightarrow> s''' = pop_frame s s'' \<Longrightarrow> \<forall>a. memory_\<alpha> s''' (haddr a) = memory_\<alpha> s'' (haddr a)"
+  by (cases s; cases s'; cases s''; cases s'''; fastforce)
+
+lemma "s' = push_frame s \<Longrightarrow> s'' = f s' \<Longrightarrow> mem_op_well_behaved f \<Longrightarrow> s''' = pop_frame s s'' \<Longrightarrow> \<forall>a. memory_\<alpha> s (saddr a) = None \<longrightarrow> memory_\<alpha> s''' (saddr a) = None"
+  apply (cases s; cases s'; cases s''; cases s''')
+  apply simp
+
+
+
 
 end
