Result.thy
@@ -8,7 +8,7 @@ section "Definitions"
 subsection "Types"
 
 datatype error = unknown_register_name
-  | unallocated_address | uninitialized_address
+  | invalid_address
   | not_an_address | incompatible_types | unknown_label
   | phi_no_previous_block | phi_label_not_found | phi_label_not_distinct
 
